fairness/examples/ticketlock/fair_lock.v
@@ -10,6 +10,7 @@ Class FairLockPredicates (M: FairModel) := {
   can_lock_st: fmrole M -> fmstate M -> Prop;
   has_lock_st: fmrole M -> fmstate M -> Prop;
   active_st: fmrole M -> fmstate M -> Prop;
+  disabled_st: fmrole M -> fmstate M -> Prop;
   is_unused: fmrole M -> fmstate M -> Prop;
   (* state_wf: fmstate M -> Prop; *)
   (* is_unused := fun ρlg st => ¬ can_lock_st ρlg st /\ ¬ has_lock_st ρlg st; *)
@@ -17,6 +18,7 @@ Class FairLockPredicates (M: FairModel) := {
   has_lock_st_dec :> forall ρ st, Decision (has_lock_st ρ st);
   can_lock_st_dec :> forall ρ st, Decision (can_lock_st ρ st);
   active_st_dec :> forall ρ st, Decision (active_st ρ st);
+  disabled_st_dec :> forall ρ st, Decision (disabled_st ρ st);
   is_unused_dec :> forall ρ st, Decision (is_unused ρ st);
 }.
 
@@ -32,14 +34,16 @@ Section FairLock.
   Definition eventual_release (tr: mtrace EFM) (ρ: R) (i: nat) :=
     forall (ρ': R) j st' (JTH: tr S!! j = Some st')
       (HAS_LOCK: has_lock_st ρ' st')
-      (DIS: ¬ role_enabled_model ρ' st')
+      (* (DIS: ¬ role_enabled_model ρ' st') *)
+      (DIS: disabled_st ρ' st')
       (AFTER: i <= j -> (ρ' ≠ ρ /\ forall k st_k (BETWEEN: i <= k <= j) (KTH: tr S!! k = Some st_k), ¬ has_lock_st ρ st_k)),
       exists k st'', tr S!! k = Some st'' /\ j <= k /\ active_st ρ' st''.
 
   Lemma eventual_release_strenghten tr ρ i (EV_REL: eventual_release tr ρ i):
     forall (ρ': R) j st' (JTH: tr S!! j = Some st')
       (HAS_LOCK: has_lock_st ρ' st')
-      (DIS: ¬ role_enabled_model ρ' st')
+      (* (DIS: ¬ role_enabled_model ρ' st') *)
+      (DIS: disabled_st ρ' st')
       (AFTER: i <= j -> (ρ' ≠ ρ /\ forall k st_k (BETWEEN: i <= k <= j) (KTH: tr S!! k = Some st_k), ¬ has_lock_st ρ st_k)),
     exists k, ClassicalFacts.Minimal
            (fun k => exists st'', tr S!! k = Some st'' /\ j <= k /\ active_st ρ' st'') k.
@@ -67,7 +71,9 @@ Section FairLock.
       (CAN_LOCK: can_lock_st ρ st)
       (ACT: active_st ρ st)
       (EV_REL: eventual_release tr ρ i),
-    exists n st', i < n /\ tr S!! n = Some st' /\ has_lock_st ρ st' /\ ¬ role_enabled_model ρ st'.
+    exists n st', i < n /\ tr S!! n = Some st' /\ has_lock_st ρ st' /\ 
+               (* ¬ role_enabled_model ρ st'. *)
+               disabled_st ρ st'. 
   
 End FairLock.
 
@@ -143,13 +149,18 @@ Class FairLock (M: FairModel) (FLP: FairLockPredicates M) (FLE: FairLockExt M) :
   allow_unlock_impl: fmrole M -> fmstate M -> fmstate M;
   allow_lock_impl: fmrole M -> fmstate M -> fmstate M;
   allows_unlock_impl_spec ρ st
-    (* (WF: state_wf st) *)
     :
     forall st', allows_unlock ρ st st' <->
-             (allow_unlock_impl ρ st = st' /\ (has_lock_st ρ st /\ ¬ active_st ρ st));
+             (allow_unlock_impl ρ st = st' /\ (has_lock_st ρ st /\ 
+                                                (* ¬ role_enabled_model ρ st *)
+                                                disabled_st ρ st
+));
   allows_lock_impl_spec ρ st:
     forall st', allows_lock ρ st st' <->
-             (allow_lock_impl ρ st = st' /\ (can_lock_st ρ st /\ ¬ active_st ρ st));
+             (allow_lock_impl ρ st = st' /\ (can_lock_st ρ st /\ 
+                                              (* ¬ role_enabled_model ρ st *)
+                                              disabled_st ρ st
+             ));
     
   (* model_step_keeps_others_preds: forall st1 ρ st2 ρ', *)
   (*   fmtrans M st1 (Some ρ) st2 -> ρ' ≠ ρ -> *)
@@ -161,8 +172,10 @@ Class FairLock (M: FairModel) (FLP: FairLockPredicates M) (FLE: FairLockExt M) :
   step_keeps_lock_dis: forall (ρ: fmrole M),
       label_kept_state
         (fun st =>
-           (* @state_wf _ FLP st /\ *)
-                  has_lock_st ρ st /\ ¬ role_enabled_model ρ st)
+                  has_lock_st ρ st /\ 
+                    (* ¬ role_enabled_model ρ st *)
+                    disabled_st ρ st
+        )
         (other_proj ρ (FLE := FLE))
         (M := @ext_model_FM _ (FL_EM FLE));
 
@@ -186,9 +199,12 @@ Class FairLock (M: FairModel) (FLP: FairLockPredicates M) (FLE: FairLockExt M) :
   (*     mkEI ∈ [flU; flL] -> @ETs _ (FL_EM FLE) (mkEI ρ) st1 st2 -> *)
   (*     forall ρ', is_unused ρ' st1 <-> is_unused ρ' st2; *)
 
-  (* TODO: is it possible to get rid of this active_st - live_roles duplication? *)
-  active_st_live: forall tl_st ρlg,
-      active_st ρlg tl_st -> ρlg ∈ live_roles _ tl_st;
+  (* (* TODO: is it possible to get rid of this active_st - live_roles duplication? *) *)
+  (* active_st_live: forall tl_st ρlg, *)
+  (*     active_st ρlg tl_st -> ρlg ∈ live_roles _ tl_st; *)
+
+  disabled_not_live: forall tl_st ρlg,
+      disabled_st ρlg tl_st -> ρlg ∉ live_roles _ tl_st;
 
   has_lock_st_excl: forall tl_st ρlg1 ρlg2,
       has_lock_st ρlg1 tl_st -> has_lock_st ρlg2 tl_st -> ρlg1 = ρlg2;
@@ -206,8 +222,8 @@ Class FairLock (M: FairModel) (FLP: FairLockPredicates M) (FLE: FairLockExt M) :
 }.
 
 
-Lemma not_live_not_active `(@FairLock M FLP FLE):
-  forall tl_st ρlg, ρlg ∉ live_roles _ tl_st -> ¬ active_st ρlg tl_st.
-Proof. 
-  intros. pose proof (active_st_live tl_st ρlg). tauto.
-Qed.
+(* Lemma not_live_not_active `(@FairLock M FLP FLE): *)
+(*   forall tl_st ρlg, ρlg ∉ live_roles _ tl_st -> ¬ active_st ρlg tl_st. *)
+(* Proof.  *)
+(*   intros. pose proof (active_st_live tl_st ρlg). tauto. *)
+(* Qed. *)
